added the Gcd Function test case.
The last line prints the result of compiling Gcd_terminate to L3.

2 Observations:

1) The environment is too big, perhaps because it contains even the
definitions that were used in the erased proof. The whole result of compilation runs into 50K lines (using Coq's Print).
This makes it very important to prune the environment in L3 to L4.
Perhaps Certicoq should take as input the functions that the user is interested in compiling, and prune everything
in the environment that is not needed to get those functions to be well-defined. This is what the current
extractor does.

2) After projecting out just the definition of Gcd_terminate, we get 900 lines in L3.
When pretty printed, this may result in a much shorter term, but the size is still concerning.

theories/allInstances.v
@@ -244,6 +244,8 @@ Print comp_fEnv6'.
 Definition comp_fEnv7 := compile_L6 comp_fEnv6.
 
 
+
+
 Quote Recursively Definition make_args := L6_to_Clight.compute_fEnv.
 Definition comp_fEnv6 : cTerm certiL6.
 (let t:= eval vm_compute in (translateTo (cTerm certiL6) comp_fEnv) in 
@@ -263,3 +265,53 @@ Require Import runtime.runtime.
 Definition test := L6_to_Clight.print_Clight_dest p7 "threePlusFour.c".
 
 Definition test2 := L6_to_Clight.print_Clight_dest runtime.runtime.prog "gc.c".
+
+
+Require Import NPeano.
+Require Import Recdef.
+Set Implicit Arguments.
+Require Import Omega.
+
+Function Gcd (a b : nat) {wf lt a} : nat :=
+match a with
+ | O => b 
+ | S k =>  Gcd (b mod S k)  (S k)
+end
+.
+Proof.
+- intros m n k Heq. subst. apply Nat.mod_upper_bound.
+  omega.
+- exact lt_wf.
+Defined.
+
+
+Quote Recursively Definition pgcd :=
+Gcd.
+
+(*
+Ltac vmcomputeExtract certiL2 f:=
+(let t:= eval vm_compute in (translateTo (cTerm certiL2) f) in 
+match t with
+|Ret ?xx => exact xx
+end).
+*)
+
+Let pcgd2 : cTerm certiL2.
+let T:= eval vm_compute in (L2.compile.program_Program pgcd) in exact T.
+Defined.
+
+Let pcgd3 : cTerm certiL3.
+(let t:= eval vm_compute in (certiClasses.translate (cTerm certiL2) (cTerm certiL3) pcgd2) in 
+match t with
+|Ret ?xx => exact xx
+end).
+Defined.
+
+(* the Gcd_terminate function is in the environment. Below,
+we project that part of the environment.
+The environment is too big, because it contains even the
+definitions that were used in the erased proof. *)
+Eval vm_compute in (nth_error (AstCommon.env pcgd2) 1).
+Eval vm_compute in (nth_error (AstCommon.env pcgd3) 1).
+
+
